src/PrimitiveDecoder/BooleanCorrectness.v
@@ -1,0 +1,23 @@
+Require Import BooleanExecSpec AbstractSpec Lib.
+Require Import Core.Core Core.Notations Core.Tactics ErrorWithWriter.
+From ExtLib.Structures Require Import Monad MonadWriter Monoid.
+From ExtLib.Data Require Import Monads.OptionMonad List.
+
+Import MonadNotation.
+
+Open Scope monad.
+
+Theorem der_encoder_correctness : forall td b ls ,
+  decoder_type td = BOOLEAN_t ->
+  execErrW (bool_encoder td b) nil = Some ls ->
+  DER (BOOLEAN b) ls.
+Admitted.
+
+Definition byte_to_bool b := if (b == 0)%byte then false else true.
+
+Theorem ber_decoder_correctness : forall td ls b z,
+    decoder_type td = BOOLEAN_t ->
+    bool_decoder td ls = Some (b, z) ->
+    BER_Bool (byte_to_bool b) (firstn (Z.to_nat z) ls).
+Admitted.
+
